lawyer/nonblocking/wfree_adequacy_lib.v
@@ -514,6 +514,122 @@ Section Lib.
       by rewrite RTH.
   Qed.
 
+  Let OP := LocaleOP (OPRE := OPP_WF) (Locale := locale heap_lang). 
+  Existing Instance OP.
+  Let OM := ObligationsModel.
+
+  Let M := AM2M ObligationsAM.
+  Let ASEM := ObligationsASEM.
+  Let EM := TopAM_EM ASEM (fun {Σ} {aGS: asem_GS Σ} _ _ => ⌜ True ⌝%I).
+
+  Definition obls_om_traces_match_wfree: extrace heap_lang -> trace (mstate M) (mlabel M) -> Prop :=
+    obls_om_traces_match_gen obls_st_rel_wfree.
+
+  Lemma obls_st_rel_wfree_empty σ (s: mstate OM)
+    (INIT: obls_is_init_st ([], σ) s):
+    obls_st_rel_wfree ([], σ) s.
+  Proof using.
+    red. 
+    rewrite /obls_st_rel /no_extra_obls.
+    rewrite /obls_fairness_preservation.om_live_tids /has_obls.
+    simpl in INIT. red in INIT.
+    rewrite /locales_of_cfg in INIT. rewrite list_to_set_nil in INIT.
+    apply proj1, eq_sym, dom_empty_inv_L in INIT.
+    rewrite INIT.
+    split; try set_solver.
+  Qed.    
+
+  Lemma int_ref_int_empty m ai σ s
+    (FITS : fits_inf_call ic m ai {tr[ ([], σ) ]})
+    (PROP : obls_st_rel_wfree ([], σ) s):
+    int_ref_inf (obls_sim_rel_wfree) ⟨ ([], σ) ⟩ ⟨ s ⟩.
+  Proof using. 
+    apply int_ref_int_singleton.
+    repeat split; try by apply PROP.
+    red. simpl. intros _ TI0.
+    assert (tctx_index ic = 0) by lia.
+    destruct FITS as [CALL _ _ _].
+    rewrite H /= in CALL.
+    rewrite /call_at /= in CALL.
+    by edestruct no_expr_in_empty_pool.
+  Qed.    
+
+  From trillium.program_logic Require Import simulation_adequacy_em_cond.
+
+  Theorem om_simulation_adequacy_model_trace_multiple_waitfree Σ
+        `{hPre: @heapGpreS Σ M EM} (s: stuckness)
+        (es: list (expr heap_lang)) σ1 (s1: mstate M) p
+        (* s' ic *)
+        m ai
+        (INIT: em_is_init_st (es, σ1) s1 (ExecutionModel := EM))
+        (extr : extrace heap_lang)
+        (Hvex : extrace_valid extr)
+        (Hexfirst : trfirst extr = (es, σ1))
+    :
+    PR_premise_multiple (obls_sim_rel_wfree ) (fits_inf_call ic m ai) Σ s es σ1 s1 (p: @em_init_param _ _ EM) ->
+    (∃ omtr, obls_om_traces_match_wfree extr omtr ∧ trfirst omtr = s1 /\
+              int_ref_inf (obls_sim_rel_wfree) extr omtr
+    ) \/
+    (exists k, ¬ (fits_inf_call ic m ai) (trace_take_fwd k extr)).
+  Proof using.
+
+    (* Set Printing Implicit. *)
+    intros PREM.
+
+    destruct (decide (1 <= length es)).
+    2: { clear PREM.
+         
+      (* TODO: make a lemma *)
+         assert (length es = 0) by lia.
+         assert (es = []) as -> by (destruct es; simpl in H; lia || done).
+         opose proof * extrace_valid_empty as ->; eauto.
+
+         destruct (decide (fits_inf_call ic m ai ({tr[ ([], σ1) ]}))) as [FITS | ].
+         2: { right. exists 0. by rewrite trace_take_fwd_0_first. }
+         
+         assert (obls_st_rel_wfree ([], σ1) s1) as PROP by (by apply obls_st_rel_wfree_empty).
+
+         left. exists (tr_singl s1).
+         clear s. 
+         split.
+         2: { split; [done| ]. by eapply int_ref_int_empty. }
+         red. by apply trace_match_singl. }
+
+    unshelve epose proof (@PR_strong_simulation_adequacy_traces_multiple _ _ EM 
+                            HeapLangEM (obls_sim_rel_wfree) (fits_inf_call ic m ai)
+                            _ _ _ _ _ 
+                            s es σ1 s1 p
+                extr
+                Hvex
+                ltac:(done)
+                obls_ves_wrapper
+                (obls_st_rel_wfree)
+                (fun oτ '(_, τ') => oτ = τ')
+                _ _ _ _ _ _ _
+                PREM
+      ) as SIM.
+    { apply fits_inf_call_prev. }
+    { simpl. intros ????[??]? STEP.
+      red in STEP. simpl in STEP. destruct STEP as [STEP ->].
+      destruct o; [| done].
+      simpl in STEP. red in STEP. apply STEP. }
+    { simpl. intros ????[??]? STEP.
+      red in STEP. simpl in STEP. destruct STEP as [STEP ->].
+      destruct o; [| done].
+      simpl in STEP. red in STEP.
+      constructor. apply STEP. }
+    { simpl. intros ?? SIM.
+      split; apply SIM. }
+    { simpl. intros ?? SIM. apply SIM. }
+    { done. }
+    { eapply adequacy_utils.rel_finitary_impl; [| apply obls_sim_rel_FB].
+      2, 3: by apply _.
+      intros ?? X. apply X. }
+    { done. }
+
+    done.
+  Qed.
+
 End Lib.
 
 Lemma fair_call_extend etr Ki Kj τ i j ci
@@ -772,5 +888,4 @@ Proof using.
     inversion NEXT. set_solver. }
   eapply mk_is_Some, state_lookup_dom in NEXT; eauto.
   simpl in *. lia.
-Qed.  
-
+Qed.
